iris/ProofSysChdir.v
@@ -110,7 +110,6 @@ Require Import InodeRegion.
 Require Import IrefSlots.
 Require Import IcacheRef.
 Require Import IcacheEscrow.
-Require Import IcacheBoot.
 Require Import FileInvDefs.
 Require Import ProcInv.
 Require Import SpecMyproc.
