iris/ProofSysOpen.v
@@ -72,7 +72,6 @@ Require Import IrefSlots.
 Require Import IcacheRef.
 Require Import IcacheInv.
 Require Import IcacheEscrow.
-Require Import IcacheBoot.
 Require Import KvmSpec.
 Require Import DirView.
 Require Import FileInvDefs.
